Clap/eDSLState/HashCons/HashConsSt.lean
@@ -2,6 +2,7 @@ import Clap.eDSLState.HashCons.CacheExpr
 
 namespace Clap
 
+@[grind]
 structure HashConsSt (p : ℕ) where
   exprs : Array (CacheExpr p) -- ℕ → Expr
   wellFormed : ∀ i < exprs.size, exprs[i]?.any (·.wellFormed i)
@@ -11,6 +12,10 @@ namespace HashConsSt
 def empty (p : ℕ) : HashConsSt p where
   exprs := #[]
   wellFormed := by simp
+
+@[simp, grind =]
+def size {p} (σ : HashConsSt p) : ℕ :=
+  σ.exprs.size
 
 instance {p} : EmptyCollection (HashConsSt p) := ⟨HashConsSt.empty p⟩
 
